---
title: "Notes (LCBB 03/07): The Power of Lambda"
author: jcb
date: 2017-12-13
tags: workthrough, math, functional-programming, lambda-calculus
---

# 3 The Power of Lambda

## 3.1 Definition of Booleans

1.  ```
    true = K
    false = K*
    ```

2.  ```
    if-then-else = (\i t e. i t e)
    ```

I think the pattern of using the "first" and "second" selector combinators
as booleans so that you can just use the truth-condition in an
"if-then-else" to directly select the right branch is really pretty somehow.

## 3.2 Definition of Pairs

```
(M, N) = (\z. z M N)

(M, N) true = M
(M, N) false = N
```

Of course, an "if-then-else" is inherently a pair: a pair of two code
branches that you switch between based on some condition. If you interpret
the branches as data branches rather than code branches, you get a really
nice representation of an ordered pair.

You can even use this pattern to construct any k-tuple. So a triple would
be:

```
(T1, T2, T3) = (\z. z T1 T2 T3)
(T1, T2, T3) (choose-of 1 3) = T1
(T1, T2, T3) (choose-of 2 3) = T2
(T1, T2, T3) (choose-of 2 3) = T3
```

Where `choose-of i n` is an expression that gives you the `i`-th expression
of `n` expressions:

```
choose-of 0 1 = \x1. x1   = I
choose-of 0 2 = \x1 x2. x1 = K
choose-of 1 2 = \x1 x2. x2 = K*
choose-of 0 3 = \x1 x2 x3. x1
choose-of 1 3 = \x1 x2 x3. x2
choose-of 2 3 = \x1 x2 x3. x3
```

How might we implement "choose of"?

Let's start with an easier function `drop` which drops the first
`n` arguments:

Well, so first lets try to build a function that adds a
layer of abstraction around any expression. So for any `M` we want:

```
(\x. M) = (\ m x . m) M = K M
```

Which is just the `K` combinator. Let's look at what happens if we apply the
`K` combinator multiple times:

```
K (K M) = K (\x. M) = (\x2. (\x1 . M)) = \x2 x1. M
K (K (K M)) = K (\x2. (\x1 . M))  = (\x3. (\x2. (\x1 . M)) = \x3 x2 x1. M
...
```

We can use the exponentiation notation from the last chapter to clean this
up:

```
K^0 M = M
K^1 M = K M
K^2 M = K (K M)
...
```

If we let `M` be the identity combinator, then we have
our `choose-n` function:

```
drop C_m = C_m K I

drop 0  = C_0 K I = I
drop 1  = C_1 K I = K I = K*
drop 2  = C_2 K I = K (K I) = (\x y z. z)
```

But if there are more than `n` arguments:

```
(T1, T2, T3) (drop 1) = (C_1 K I) T1 T2 T3 = K* T1 T2 T3 = T2 T3
```

So our `choose-of` function is going to need to get rid of a bunch of
arguments that come after the one we want.

Let's define another function `first n` that returns the first of `n + 1`
arguments.


```
first 0 = \ x1. x1
first 1 = \ x1 x2. x1
first 2 = \ x1 x2 x3. x1
...
```

By a similar construction to `drop`:

```
first C_n = \x . C_n K x
first 0 = \x . x
first 1 = \x . K x
first 2 = \x . K (K x)
...
```

Let's test this out:

```
(T1, T2, T3) (first 2) = (\x . K (K x)) T1 T2 T3
= K (K T1) T2 T3
= (K T1) T3
= T1
```

So our `choose-of` function will be:

```
choose-of = \ i n t. (first (sub n i)) (t (drop i))
```

Where `sub` is integer subtraction, whose derivation I'll leave for elsewhere.

[TODO: Subtraction]

Honestly, this construction of `n`-tuples seems ugly, and I'm not the biggest
fan of writing lambda expressions that are complicated enough to feel
like actual code. If I'm going to write code I want some actual tools...


## 3.3 Definition of natural numbers as pairs

```
0_ = I
(n + 1)_ = (false, n_)
```

So numbers can be defined as nested pairs.

## 3.4 Lemma: Successor, predecessor, isZero

```
succ n_ = (n + 1)_ = (false, n_)
succ = (\n. (\p. p false n))

pred (n+1) = (\n. n false) (\p. p false n_)  = false false n_ = n_
pred = (\n. n false)

isZero = (\x . x true)
isZero 0 = (\x . x true) I = true
isZero 1 = (\x . x true) (\ p. p false n_) = true false n_ = false
```


## 3.5 Definition
